\documentclass{article}
\usepackage{amsmath}
\usepackage{multicol}
\usepackage{blindtext}
\usepackage{geometry}
\usepackage{makecell}
 \geometry{
 a4paper,
 left=10mm,
 top=10mm,
 right=10mm,
 bottom=10mm,
 }
\usepackage{enumitem}
\setlist[itemize]{align=parleft,left=0pt..1em}
\begin{document}
\thispagestyle{empty}

\begin{multicols*}{2}

  \noindent\textbf{Harmonic Motion}
  \begin{itemize}
    \item $A \sin(\omega t + \phi)$
    \item $A \exp^{i(\omega t + \phi)} = A(\cos(\omega t + \phi) + i\sin(\omega t + \phi))$
  \end{itemize}

  \noindent\textbf{Second Order Differential Equation}
  \begin{itemize}
  \item when $b^2 - 4ac > 0$, two different roots $r_1, r_2$, $y = C_1\exp^{r_1 x} + C_2\exp^{r_2 x}$
  \item when $b^2 - 4ac = 0$, two equal roots $r$, $y = C_1 e^{r x} + C_2 x e^{r x}$
  \item when $b^2 - 4ac < 0$, two equal roots $a \pm bi$, $y = e^{ax} [C_1 \cos(b x) + C_2 \sin(b x)]$
  \end{itemize}

  \noindent\textbf{EOM of M-DOF}
  \begin{itemize}
  \item $[M]\{\ddot{q}\} + [c]\{\dot{q}\} + [K]\{q\}=\{F\}$
  \item For a static system, $\{\dot{q} = \ddot{q} = 0\}$, $[K]\{q\}=\{F\}$.
  \item How to get Natural Frequency? => When external force and damping to 0:
    $[M]\{\ddot{q}\} + [K]\{q\} = 0$, $\{q\} = \{\bar{q}\}\exp^{i\omega t}$, thus $\omega^2 = [M^{-1}][K]$.
  \end{itemize}

  \noindent\textbf{Forced Vibration}
  \begin{itemize}
  \item For Harmonic force $F\sin\omega t$, EOM: $m\ddot{x} + c\dot{x} + kx = F\sin\omega t$, $x_t = \frac{F/k}{\sqrt{(1-r^2)^2+(2\xi r)^2}}\sin(\omega t + \phi)$, $r=\frac{\omega}{\omega_n}$
    \item
  \item EOM $x = \int_0^t F(\xi) h(t-\xi) d\xi$
  \item Impulsive response $h(t) = \frac{1}{M\omega_n}\sin(\omega_n t)$
  \end{itemize}

  \noindent\textbf{Virtual Work}
  \begin{itemize}
  \item The virtual work of a static system is always 0.
  \item D'Alembert's Principle
    \begin{equation*}
      \sum_k (F_k - m \ddot{r_k}) \delta r_k = 0
    \end{equation*}
  \end{itemize}

  \noindent\textbf{Quantities}
  \begin{itemize}
  \item Torque $\tau = Fr \sin\theta$
  \item Rotational Inertia $I=\frac{1}{2}mr^2$ (For rigid)
  \item Rotational Torque $\tau = I\alpha$, $\alpha = \dot{\omega}$
  \item Rotational Kinetic Energy $E_{rotational}=\frac{1}{2}I\omega^2$
  \end{itemize}

  \noindent\textbf{Lagrange Equation}
  \begin{equation*}
    \frac{d}{dt}\frac{dT}{d\dot{q_i}} - \frac{dT}{dq_i} + \frac{dU}{dq_i} = 0
  \end{equation*}

  \noindent\textbf{Elasticity}
  \begin{itemize}
  \item \textbf{Stress $\sigma$} distribution of internal force within a body $\frac{F}{A}$
  \item \textbf{Stain $\varepsilon$} deformation within a body $\frac{\Delta L}{L}$
  \item \textbf{Young's Modulus $E$} In elastic region, $\sigma = E\varepsilon$
  \item \textbf{Shear Force $\tau$} conduct by transverse force $\frac{F}{A}$
  \end{itemize}
  Hook's law
  \begin{equation*}
    \sigma=\frac{N}{s}=E\varepsilon=E\frac{\partial u}{\partial x}
  \end{equation*}

  \noindent\textbf{Beam}
  \begin{itemize}
  \item Given point $(x_1, 0, 0, t)$, $u_i(x_1, x_2, x_3, t) = u_i^0(x_1,t) + u_i^2(x_1,t) + u_i^3(x_1,t)$
  \item $u_i^0$ Transitional displacement
  \item $u_2^1, u_3^1$ Rotational displacement
  \item $u_3^2, u_2^3$ Torsion displacement
  \item $u_2^2, u_3^3$ Poisson displacement
  \item \textbf{Longitudinal} For small part $dx$ of beam, $\partial u$ is the displacement of $dx$, EOM is
    \begin{equation*}
      f(x) + \frac{\partial}{\partial x}(ES\frac{\partial u}{\partial x} -\rho S\frac{\partial^2 u}{\partial t^2}) = 0
    \end{equation*}
    BC:
    \begin{itemize}
    \item Free end: $N=0, \sigma=0$, $\frac{\partial u}{\partial x}\mid_{x=0 \text{ or } L} = \sigma = 0$
    \item Fixed end: $u\mid_{x=0 \text{ or } = L} = 0$
    \end{itemize}
    Kinetic Energy: $T = \inf_v \frac{1}{2} \rho (\frac{\partial u}{\partial t})^2 dv$\\
    Potential Energy: $U = \inf_v \frac{1}{2}\sigma_{ij} \epsilon_{ij} dv$

  \item\textbf{Flexural}
    \begin{itemize}
    \item \textbf{Momentum} $EI\frac{\partial w}{\partial x}$
    \item \textbf{Rotation} $\frac{\partial w}{\partial x}$
    \item \textbf{Displacement} $w$
    \item \textbf{Shear Force} $\frac{\partial M}{\partial x}$
    \item \textbf{Kinetic Energy} $T = \frac{1}{2}\int_v\rho (\frac{\partial u_i}{\partial t})^2 dv$
    \item \textbf{Potential Energy} $U = \frac{1}{2} \int_v \sigma_{ij} \epsilon_{ij} dv = \frac{1}{2} \int_l EI(\frac{\partial^2 w}{\partial x^2})^2 dx$
    \item EOM
      \begin{equation*}
        \frac{\partial}{\partial x^2} EI\frac{\partial^2 w}{\partial x^2} + \rho S \frac{\partial^2 w}{\partial t^2} = -f - \frac{\partial m}{\partial x}
      \end{equation*}
    \item When no force: $w = A\cos\alpha x + B\sin\alpha x + C\cosh\alpha x + D\sinh\alpha x$, $\alpha^4 = \frac{\rho S \omega^2}{EI}$
    \item \textbf{BC}
      \begin{itemize}
      \item Simply-Supported $w \mid_{0 \text{ and } l} = 0$, $\frac{\partial^2 w}{\partial x^2} \mid_{0 \text{ and } l} = 0$
      \item Clamped-Clamped $w \mid_{0 \text{ and } l} = 0$, $\frac{\partial w}{\partial x} \mid_{0 \text{ and } l} = 0$
      \item Free-Free $\frac{\partial^2 w}{\partial x^2} \mid_{0 \text{ and } l} = 0$
      \item Clamped-Free
      \end{itemize}
    \item \textbf{Rayleigh method} Since $T_{max} = U_{max}$, assume $w(x,t) = y(x) \sin\omega t$,
      \begin{equation*}
        \omega^2 = \int_0^l EI(\frac{d^2y}{dx^2})^2 dx / \int_0^l \rho s y^2 dx)
      \end{equation*}
      This method is more accurate if assumed function $y(x,t)$ \textbf{satisfy} all BCs.

    \item \textbf{Ritg method}
      \begin{enumerate}
      \item Decompose $w(x,t) = a_0(t) + a_1(t)x + a_2(t)x^2$
      \item Use BC to simplied $w(x,t)$
      \item Calculate $T$ and $U$
      \item Solve Lagrange $L = T - U$, get $\omega$ and mode shape
      \end{enumerate}
    \end{itemize}
  \end{itemize}

  \noindent\textbf{Hamilton's Principle}
  \begin{equation*}
    H=\int_{t_{1}}^{t_{2}}(T-V+W_{F})\text{d}t
    =\int_{t_{1}}^{t_{2}}\int_{0}^{L}F(u,u_{,t},u_{,x})\text{d}x\text{d}t
  \end{equation*}

  \noindent\textbf{Eular Equation}
  \begin{equation*}
    \frac{\partial F}{\partial u}-\frac{\partial}{\partial x}(\frac{\partial F}{\partial u_{,x}})-\frac{\partial}{\partial t}(\frac{\partial F}{\partial u_{,t}})=0
  \end{equation*}

  \noindent\textbf{Plate}
  \begin{itemize}
  \item Love-Kirchoff plates assumptions:
    \begin{enumerate}
    \item neglect deformation along thickness direction (poison effect, $u_3^3=0$)
    \item neglect in-plane motion $u_1^0=u_2^0=0$
    \end{enumerate}
  \end{itemize}




%%%%%%%%%%%%%%%%%%%%%%%%%%%%%%%%%%%%%%%%%%%%%%%%%%%%%%%%%%%%%%%%%%%%%%%%%%%%%%%%
  \begin{table*}
    \centering
    \caption{comparison}
    \begin{tabular}{|c|c|c|c|c|}
      \hline
      Name&string&Longitudinal beam& Flexural beam&plate\\
      \hline
      T&$\frac{1}{2}\int_{0}^{l}m(x)(\frac{\partial y}{\partial t})^{2}\text{d}x$
      &$\frac{1}{2}\int_{0}^{l}\rho s(\frac{\partial u}{\partial t})^{2}\text{d}x$
      &$\frac{1}{2}\int_{0}^{l}\rho s(\frac{\partial u}{\partial t})^{2}\text{d}x$
      &$\frac{1}{2}\int_{0}^{l_{1}}\int_{0}^{l_{2}}\rho h(\frac{\partial w}{\partial t})^{2}\text{d}x_{1}\text{d}x_{2}$\\
      \hline
      V&$\frac{1}{2}\int_{0}^{l}T(\frac{\partial y}{\partial x})^{2}\text{d}x$
      &$\frac{1}{2}\int_{0}^{l}Es(\frac{\partial^{2} w}{\partial x^{2}})^{2}\text{d}x$
      &$\frac{1}{2}\int_{0}^{l}EI(\frac{\partial^{2} w}{\partial x^{2}})^{2}\text{d}x$
      &$\frac{1}{2}\int_{v}\sigma_{ij}\varepsilon_{ij} \text{d}$v\\
      \hline
      Motion Equation&$T\frac{\partial ^{2}y(x,t)}{\partial x^{2}}=m(x)\frac{\partial^{2}y(x,t)}{\partial t^{2}}$
      &$\frac{\partial^{2}u(x,t)}{\partial x^{2}}-\frac{\rho}{E}\frac{\partial^{2}u}{\partial t^{2}}=0$
      &\makecell[c]{$\frac{\partial ^{2}}{\partial x^{2}}(EI\frac{\partial^{2}w}{\partial x^{2}})+\rho s \frac{\partial^{2}w}{\partial t^{2}}=$ \\ $-f(x,t)-\frac{\partial m(x,t)}{\partial x}$}
      &\makecell[c]{$D \bigtriangledown ^{4}w+\rho h \frac{\partial ^{2}}{\partial t^{2}}=f$\\
      $D=\frac{Eh^{3}}{12(1-v^{2})}$\\$\bigtriangledown^{4}=\frac{\partial ^{4}}{\partial x_{1}^{4}}+2\frac{\partial ^{4}}{\partial x_{1}^{2}\partial x_{2}^{2}}+\frac{\partial ^{4}}{\partial x_{2}^{4}}$}\\
      \hline
    \end{tabular}
  \end{table*}

  \begin{table*}
    \centering
    \caption{displacement filed}
    \begin{tabular}{|c|c|c|c|}
      \hline
      general beam & logituditnal beam  & Flexural beam & plate\\
      \hline
      \makecell[c]{
        $u_{1}(x_{1},x_{2},x_{3},t)=u_{1}^{0}(x_{1},0,0,t)+$\\$x_{2}u_{1}^{2}(x_{1},0,0,t)+x_{3}u_{1}^{3}(x_{1},0,0,t)$\\
        $u_{2}(x_{1},x_{2},x_{3},t)=u_{2}^{0}(x_{2},0,0,t)+$\\$x_{2}u_{2}^{2}(x_{1},0,0,t)+x_{3}u_{2}^{3}(x_{1},0,0,t)$\\
        $u_{3}(x_{1},x_{2},x_{3},t)=u_{3}^{0}(x_{3},0,0,t)+$\\$x_{2}u_{3}^{2}(x_{1},0,0,t)+x_{3}u_{3}^{3}(x_{1},0,0,t)$\\
        $x_{2}u_1^2, x_{3}u_1^3$ Rotation \\
        $x_{2}u_3^2, x_{3}u_2^3$ Torsion \\
        $x_{2}u_2^2, x_{3}u_3^3$ Poisson
      }
      &\makecell[c]{
        $u_{1}(x_{1},x_{2},x_{3},t)=$\\$u_{1}^{0}(x_{1},0,0,t)$\\
        $u_{2}(x_{1},x_{2},x_{3},t)=0$\\
        $u_{3}(x_{1},x_{2},x_{3},t)=0$\\
      }
      &\makecell[c]{
        $u_{1}(x_{1},x_{2},x_{3},t)=x_{2}u_{1}^{2}(x_{1},t)$\\
        $u_{2}(x_{1},x_{2},x_{3},t)=u_{2}^{0}(x,t)$\\
        $u_{3}(x_{1},x_{2},x_{3},t)=0$\\
        for Bernoulli beam \\
        $u_{1}^{2}(x,t)=-\frac{\partial u_{2}^{0}}{\partial x}(x,t)$
      }
      &\makecell[c]{
        $u_{1}(x_{1},x_{2},x_{3},t)=x_{3}u_{1}^{3}(x_{1},x_{2},t)$\\
        $u_{2}(x_{1},x_{2},x_{3},t)=x_{3}u_{2}^{3}(x_{1},x_{2},t)$\\
        $u_{3}(x_{1},x_{2},x_{3},t)=u_{3}^{0}(x_{1},x_{2},t)$\\
        Love-Kirchoff plate\\
        $u_{1}=-x_{3}\frac{\partial w}{\partial x_{1}}$\\
        $u_{2}=-x_{3}\frac{\partial w}{\partial x_{2}}$\\
        $u_{3}=w$
      }\\
      \hline
    \end{tabular}
  \end{table*}

\end{multicols*}

\end{document}
